theories/Monads.v
@@ -9,18 +9,18 @@ Require Import String.
 
 (** An option type with an error message argument for the failure case,
     similar to a result *)
-Inductive optionE (X:Type) : Type :=
-  | SomeE (x : X)
-  | NoneE (s : string).
-Arguments SomeE {X}.
-Arguments NoneE {X}.
+Inductive result (X:Type) : Type :=
+  | Ok (x : X)
+  | Error (s : string).
+Arguments Ok {X}.
+Arguments Error {X}.
 
 Declare Scope monad_scope.
 Open Scope monad_scope.
 
 Notation " x <- e1 ;; e2" := (match e1 with
-                              | SomeE x => e2
-                              | NoneE err => NoneE err
+                              | Ok x => e2
+                              | Error err => Error err
                               end)
          (right associativity, at level 60) : monad_scope.
 Notation " let* '_' <= e1 #; e2 " := (match e1 with
@@ -28,17 +28,17 @@ Notation " let* '_' <= e1 #; e2 " := (match e1 with
                                     end)
          (right associativity, at level 60) : monad_scope.
 Notation " 'return' e "
-  := (SomeE e) (at level 60) : monad_scope.
+  := (Ok e) (at level 60) : monad_scope.
 Notation " 'fail' s "
-  := (NoneE s) (at level 60) : monad_scope.
+  := (Error s) (at level 60) : monad_scope.
 
-(** Attempt to convert a list of [optionE]s to a list of the [SomeE] contents,
-    fails on the first [NoneE] *)
-Fixpoint strip_options {X : Type} (l : list (optionE X)) : optionE (list X) :=
+(** Attempt to convert a list of [result]s to a list of the [Ok] contents,
+    fails on the first [Error] *)
+Fixpoint strip_options {X : Type} (l : list (result X)) : result (list X) :=
   match l with
   | nil => return nil
-  | cons (SomeE a) t =>
+  | cons (Ok a) t =>
     t' <- strip_options t ;;
     return (cons a t')
-  | cons (NoneE s) _ => fail ("strip_options fail: " ++ s)
+  | cons (Error s) _ => fail ("strip_options fail: " ++ s)
   end.
