theories/Server.v
@@ -36,7 +36,7 @@ Definition server_username : username.
         NoSpaces := H0 |}.
 Defined.
 
-Definition server_client_communication (uname : username) (cc : client_connection) : optionE unit :=
+Definition server_client_communication (uname : username) (cc : client_connection) : result unit :=
     (* Add the new connection *)
     let* _ <= log Log_Info (uname.(Uname) ++ " has joined") #;
     let cc := {|
@@ -56,7 +56,7 @@ Definition server_client_communication (uname : username) (cc : client_connectio
         match client_msg with
         | MESG msg =>
             let* _ <= log Log_Info (cc.(cc_uname).(Uname) ++ ": " ++ msg) #;
-            _ <- SomeE (List.map (fun conn =>
+            _ <- Ok (List.map (fun conn =>
                 (* Don't send a message to the user that sent it *)
                 if conn.(cc_uname) =? uname then
                     return tt
@@ -71,7 +71,7 @@ Definition server_client_communication (uname : username) (cc : client_connectio
             target_cc <-
                 match List.filter
                     (fun cc => cc.(cc_uname) =? uname) (get_connection_list tt) with
-                | [cc] => SomeE cc
+                | [cc] => Ok cc
                 | _ => 
                     _ <- send_message cc.(cc_descr) 
                         (serialize_server_message (ERR PmsgTargetNotExists)) ;;
@@ -81,14 +81,14 @@ Definition server_client_communication (uname : username) (cc : client_connectio
                     (serialize_server_message (MSG cc.(cc_uname) ("[PM] " ++ msg))) ;;
             return log Log_Info (cc.(cc_uname).(Uname) ++ ": " ++ "[PM] " ++ msg))
             with
-            | SomeE _ => return Recurse
-            | NoneE s =>
+            | Ok _ => return Recurse
+            | Error s =>
                 let* _ <= log Log_Error s #;
                 return Recurse
             end
         | EXIT _uname =>
             let* _ <= remove_connection cc #;
-            _ <- SomeE (List.map
+            _ <- Ok (List.map
                 (fun cc => send_message cc.(cc_descr) (serialize_server_message 
                     (MSG server_username 
                     (uname.(Uname) ++ " has left"))))
@@ -101,11 +101,11 @@ Definition server_client_communication (uname : username) (cc : client_connectio
 
 (** Do initial processing of client connection, and then start communicating
     with the client *)
-Definition init_client_comms (cc : client_connection) : optionE unit :=
+Definition init_client_comms (cc : client_connection) : result unit :=
     let* _ <= log Log_Debug "Accepted new connection" #;
     (* Read 33 bytes - should be a REG message *)
     match (recv_client_message cc.(cc_descr)) with
-    | SomeE (REG uname) =>
+    | Ok (REG uname) =>
         match get_connection uname with
         (* Username is not taken *)
         | None =>
@@ -122,7 +122,7 @@ Definition init_client_comms (cc : client_connection) : optionE unit :=
                 (serialize_server_message (ERR UsernameTaken)) ;;
             return tt
         end
-    | NoneE s =>
+    | Error s =>
         let* _ <= log Log_Error s #;
         return tt
     | _ => 
@@ -134,17 +134,17 @@ Definition init_client_comms (cc : client_connection) : optionE unit :=
 (**
     Accept new connections and spawn synchronization threads for each of them
 *)
-Definition server_accept_thread (socket_fd : file_descr) : optionE unit :=
+Definition server_accept_thread (socket_fd : file_descr) : result unit :=
     repeat_until_timeout max_int (fun _ =>
         let '(client_descr, client_addr) := accept socket_fd in
         let* _ <= log Log_Debug 
             ("Accepted client socket " ++ (string_of_socket_addr client_addr)) #;
-        _ <- create client_connection (optionE unit) init_client_comms
+        _ <- create client_connection (result unit) init_client_comms
             {|cc_uname := dummy_username; cc_descr := client_descr; cc_addr := client_addr|} ;;
         return Recurse
     ).
 
-Definition server_control_thread (_ : unit) : optionE unit :=
+Definition server_control_thread (_ : unit) : result unit :=
     repeat_until_timeout max_int (fun _ => 
         command <- read_line tt ;;
         if ((command =? "exit") || (command =? "quit"))%string then
@@ -156,7 +156,7 @@ Definition server_control_thread (_ : unit) : optionE unit :=
 (**
     Wraps up all server logic: port binding, threading, etc.
 *)
-Definition server (host : string) (portno : port) : optionE unit :=
+Definition server (host : string) (portno : port) : result unit :=
     let* _ <= init_connections tt #;
     (* Create a TCP socket *)
     let socket_fd := socket PF_INET SOCK_STREAM 0 in
@@ -168,8 +168,8 @@ Definition server (host : string) (portno : port) : optionE unit :=
     (* Wait for and accept any incoming TCP connection requests. *)
     let* _ <= listen socket_fd 10 #;
     let* _ <= log Log_Info "Server started" #;
-    accept_thread <- create file_descr (optionE unit) server_accept_thread socket_fd ;;
-    control_thread <- create unit (optionE unit) server_control_thread tt ;;
+    accept_thread <- create file_descr (result unit) server_accept_thread socket_fd ;;
+    control_thread <- create unit (result unit) server_control_thread tt ;;
     let* _ <= join control_thread #;
     let* _ <= log Log_Info "Closing server" #;
     let* _ <= close socket_fd #;
